feat: rewritePeepholeRecursively (#410)
@tobiasgrosser spotted that 'rewritePeephole' only works at one level of
the IR,
and will not recurse into regions.
We write a variant ('rewritePeepholeRecursively').
This first calls 'rewritePeephole' on the 'Com'.
Then, it recurses into each let-binding of the 'Com' to call
'rewritePeepholeRecursively' on all region arguments.
This ensures that the rewrite is applied to all occurrences of the lhs
in all (nested) regions.

This supercedes https://github.com/opencompl/lean-mlir/pull/408

SSA/Projects/PaperExamples/PaperExamples.lean
@@ -227,6 +227,11 @@ instance : TyDenote Ty where
   toType
     | .int => BitVec 32
 
+instance : Inhabited (TyDenote.toType (t : Ty)) where
+  default := by
+    cases t
+    exact (0#32)
+
 inductive Op :  Type
   | add : Op
   | const : (val : ℤ) → Op
@@ -285,6 +290,7 @@ def iterate {Γ : Ctxt _} (k : Nat) (input : Var Γ int) (body : Com SimpleReg [
 
 attribute [local simp] Ctxt.snoc
 
+namespace P1
 /-- running `f(x) = x + x` 0 times is the identity. -/
 def lhs : Com SimpleReg [int] .pure int :=
   Com.var (iterate (k := 0) (⟨0, by simp[Ctxt.snoc]⟩) (
@@ -354,5 +360,98 @@ theorem EX1' : ex1' = (
   Com.ret ⟨2, by simp [Ctxt.snoc]⟩)
   := by rfl
 -/
+
+end P1
+
+namespace P2
+
+/-- running `f(x) = x + 0` 0 times is the identity. -/
+def lhs : Com SimpleReg [int] .pure int :=
+  Com.var (cst 0) <| -- %c0
+  Com.var (add ⟨0, by simp[Ctxt.snoc]⟩ ⟨1, by simp[Ctxt.snoc]⟩) <| -- %out = %x + %c0
+  Com.ret ⟨0, by simp[Ctxt.snoc]⟩
+
+def rhs : Com SimpleReg [int] .pure int :=
+  Com.ret ⟨0, by simp[Ctxt.snoc]⟩
+
+def p2 : PeepholeRewrite SimpleReg [int] int:=
+  { lhs := lhs, rhs := rhs, correct := by
+      rw [lhs, rhs]
+      funext Γv
+      simp_peephole [add, cst] at Γv
+      /-  ∀ (a : BitVec 32), a + BitVec.ofInt 32 0 = a -/
+      intros a
+      simp only [ofInt_zero, ofNat_eq_ofNat, BitVec.add_zero, BitVec.zero_add]
+  }
+
+/--
+example program that has the pattern 'x + 0' both at the top level,
+and inside a region in an iterate. -/
+def egLhs : Com SimpleReg [int] .pure int :=
+  Com.var (cst 0) <|
+  Com.var (add ⟨0, by simp[Ctxt.snoc]⟩ ⟨1, by simp[Ctxt.snoc]⟩) <| -- %out = %x + %c0
+  Com.var (iterate (k := 0) (⟨0, by simp[Ctxt.snoc]⟩) (
+      Com.letPure (cst 0) <|
+      Com.letPure (add ⟨0, by simp[Ctxt.snoc]⟩ ⟨1, by simp[Ctxt.snoc]⟩) -- fun x => (x + x)
+      <| Com.ret ⟨0, by simp[Ctxt.snoc]⟩
+  )) <|
+  Com.ret ⟨0, by simp[Ctxt.snoc]⟩
+
+/--
+info: {
+  ^entry(%0 : ToyRegion.Ty.int):
+    %1 = ToyRegion.Op.const 0 : () → (ToyRegion.Ty.int)
+    %2 = ToyRegion.Op.add (%1, %0) : (ToyRegion.Ty.int, ToyRegion.Ty.int) → (ToyRegion.Ty.int)
+    %3 = ToyRegion.Op.iterate 0 (%2) ({
+      ^entry(%0 : ToyRegion.Ty.int):
+        %1 = ToyRegion.Op.const 0 : () → (ToyRegion.Ty.int)
+        %2 = ToyRegion.Op.add (%1, %0) : (ToyRegion.Ty.int, ToyRegion.Ty.int) → (ToyRegion.Ty.int)
+        return %2 : (ToyRegion.Ty.int) → ()
+    }) : (ToyRegion.Ty.int) → (ToyRegion.Ty.int)
+    return %3 : (ToyRegion.Ty.int) → ()
+}
+-/
+#guard_msgs in #eval egLhs
+
+def runRewriteOnLhs : Com SimpleReg [int] .pure int :=
+  (rewritePeepholeRecursively (fuel := 100) p2 egLhs).val
+
+/--
+info: {
+  ^entry(%0 : ToyRegion.Ty.int):
+    %1 = ToyRegion.Op.const 0 : () → (ToyRegion.Ty.int)
+    %2 = ToyRegion.Op.add (%1, %0) : (ToyRegion.Ty.int, ToyRegion.Ty.int) → (ToyRegion.Ty.int)
+    %3 = ToyRegion.Op.iterate 0 (%0) ({
+      ^entry(%0 : ToyRegion.Ty.int):
+        %1 = ToyRegion.Op.const 0 : () → (ToyRegion.Ty.int)
+        %2 = ToyRegion.Op.add (%1, %0) : (ToyRegion.Ty.int, ToyRegion.Ty.int) → (ToyRegion.Ty.int)
+        return %0 : (ToyRegion.Ty.int) → ()
+    }) : (ToyRegion.Ty.int) → (ToyRegion.Ty.int)
+    return %3 : (ToyRegion.Ty.int) → ()
+}
+-/
+#guard_msgs in #eval runRewriteOnLhs
+
+def expectedRhs : Com SimpleReg [int] .pure int :=
+  Com.var (cst 0) <|
+  Com.var (add ⟨0, by simp[Ctxt.snoc]⟩ ⟨1, by simp[Ctxt.snoc]⟩) <| -- %out = %x + %c0
+  -- | Note that the argument to 'iterate' is rewritten.
+  -- This is a rewrite that fires at the top level.
+  Com.var (iterate (k := 0) (⟨2, by simp[Ctxt.snoc]⟩) (
+      Com.letPure (cst 0) <|
+      Com.letPure (add ⟨0, by simp[Ctxt.snoc]⟩ ⟨1, by simp[Ctxt.snoc]⟩)
+      -- | See that the rewrite has fired in the nested region for 'iterate',
+      -- and we directly return the block argument.
+      <| Com.ret ⟨2, by simp[Ctxt.snoc]⟩
+  )) <|
+  Com.ret ⟨0, by simp[Ctxt.snoc]⟩
+
+theorem rewriteDidSomething : runRewriteOnLhs ≠ lhs := by
+  simp [runRewriteOnLhs, lhs]
+  native_decide
+
+theorem rewriteCorrect : runRewriteOnLhs = expectedRhs := by rfl
+
+end P2
 
 end ToyRegion
